src/crypto/loopunroll/loopunroll.s.dfy
@@ -21,40 +21,4 @@ lemma lemma_BitwiseAdd64()
     reveal_BitwiseAdd64();
 }
 
-predicate ValidDstAddr64(h:Heaplets, id:heaplet_id, addr:int)
-{
-  id in h  && h[id].Heaplet64?   && addr in h[id].mem64
-}
-
-predicate ValidSrcAddr64(h:Heaplets, id:heaplet_id, addr:int, taint:taint) 
-{
- id in h  && h[id].Heaplet64?   && addr in h[id].mem64 && h[id].mem64[addr].t == taint
-}
-
-lemma lemma_ValidDstAddr64(mem:Heaplets, id:heaplet_id, addr : uint64)
-      requires ValidDstAddr64(mem, id, addr);
-      ensures id in mem;
-      ensures mem[id].Heaplet64?;
-      ensures addr in mem[id].mem64;
-{
-}
-
-lemma lemma_ValidSrcAddr64(mem:Heaplets, id:heaplet_id, addr : uint64, t:taint)
-      requires ValidSrcAddr64(mem, id, addr, t); 
-      ensures id in mem;
-      ensures mem[id].Heaplet64?;
-      ensures addr in mem[id].mem64;
-      ensures addr in mem[id].mem64;
-      ensures mem[id].mem64[addr].t == t;
-      ensures ValidDstAddr64(mem, id, addr);
-{
-}
-
-predicate Mem64ChangedOnlyAtWith(mem: Heaplets, old_mem : Heaplets, id : heaplet_id, 
-             addr : uint64, off : uint64, value : uint64, t : taint)
-    requires ValidSrcAddr64(old_mem, id, addr + off, Public); 
-{
-  mem == old_mem[id := old_mem[id].(mem64 := old_mem[id].mem64[addr + off := Heaplet64Entry(value, t)])]
-} 
-
 }
