src/crypto/loopunroll/proof.dfy
@@ -1,0 +1,36 @@
+include "../../lib/util/types.s.dfy"
+include "../../lib/util/operations.s.dfy"
+include "../../lib/util/words_and_bytes.s.dfy"
+include "../../lib/collections/Seqs.s.dfy"
+include "../../arch/x64/def.s.dfy"
+include "../../arch/x64/vale.i.dfy"
+include "../../lib/util/dafny_wrappers.i.dfy"
+include "addrlogic.s.dfy"
+
+module proof {
+
+import opened x64_def_s
+import opened types_s
+import opened x64_vale_i
+import opened dafny_wrappers_i
+import opened addrlogic
+
+lemma lemma_OnlyAddrs64ModifiedExt(mem0 : Heaplets, mem1 : Heaplets, mem2: Heaplets, id:heaplet_id, 
+                                   addr : uint64, count : nat) 
+  requires OnlyAddrs64Modified(mem0, mem1, id, addrs64(addr, count));
+  requires OnlyAddr64Modified (mem1, mem2, id, addroff64(addr, count + 1));
+  ensures  OnlyAddrs64Modified(mem0, mem2, id, addrs64(addr, count + 1));
+{
+  assert id in mem0 && id in mem1 && id in mem2;
+  assert ValidDstUnAddrs64(mem0, id, addrs64(addr, count));
+  assert ValidDstUnAddr64(mem1, id, addroff64(addr, count + 1));
+
+  assume ValidDstUnAddrs64(mem0, id, addrs64(addr, count + 1));
+  assume (forall naddr : int ::
+   (naddr in mem0[id].mem64 && naddr in mem2[id].mem64 && 
+    (naddr < addr || naddr > addr + count * 8)) ==>
+     mem2[id].mem64[naddr] == mem0[id].mem64[naddr]);
+}
+
+
+}
